First-cut pair automata partition.

src/dafny/utils/Automata.dfy
@@ -13,7 +13,7 @@
  */
 
 include "./MiscTypes.dfy"
-include "./int.dfy"
+include "./Partition.dfy"
 
 /** 
   * Provides finitie automata.
@@ -21,245 +21,88 @@ include "./int.dfy"
 module Automata {
 
   import opened MiscTypes
-  import Int
+  import opened PartitionMod
 
-  datatype Node<T> =
-      Num(index: nat, prop: T)
-    | Sink()
+  //   datatype Node<T> =
+  //       Num(index: nat, prop: T)
+  //     | Sink()
 
-  datatype Edge<U> = Edge(src: nat, lab: U, tgt: nat)
+  //   datatype Edge<U, T> = Edge(src: U, lab: U, tgt: T)
 
   /** Deterministic transition relation. 
     *
     *   0 is the starting state. A sink state is a state that is not
     *   in the map.   
     */
-  type Transitions = map<(nat, bool), nat>
+  //   type Transitions = map<(nat, bool), nat>
 
-  type Transitions2<T(==)> = map<(T, bool), T>
+  //   type Transitions2<T(==)> = map<(T, bool), T>
 
+  //   datatype Auto = Auto(numStates: nat, tr: Transitions, final: nat := 0)
 
-  //   predicate IsDeterministic(tr: Transitions)
-  //   {
-  //     forall k, k':: k in tr.Keys && k' in tr.Keys  ==>
-  //                      k.0 == k'.0 ==> k.1 != k'.1
-  //   }
+  //   datatype Auto2<T> = Auto2(init: T, tr: Transitions2<T>, refSet: set<T>, bound: nat)
 
-  datatype Auto = Auto(numStates: nat, tr: Transitions, final: nat := 0)
+  //   type ValidAuto2 = a: Auto2<nat> | IsBounded(a.refSet, a.bound) witness Auto2(0, map[], {}, 0)
 
-  datatype Auto2<T> = Auto2(init: T, tr: Transitions2<T>, refSet: set<T>, bound: nat)
+  //   type ValidAuto = a: Auto |
+  //       && forall k:: k in a.tr.Keys ==> k.0 < a.numStates
+  //                                        && forall k:: k in a.tr.Values ==> k < a.numStates
+  //     witness Auto(0, map[], 0)
 
+  //   state -> list of labels (enabled)
+  //  state and for each l in list of labels -> state
 
-  
-  type ValidAuto2 = a: Auto2<nat> | IsBounded(a.refSet, a.bound) witness Auto2(0, map[], {}, 0)
+  //  states = ["toto", "titi"] numbered from 0 to n
+  //  labels same: ["l0", "l1", ] numbered from 0 to k
+  //  transitions: if "titi" -- l -> "toto" then write it as 1 - i -> 0
+  //  each l in labels[i] give the labels enables in states[i]
 
-  type ValidAuto = a: Auto |
-      && forall k:: k in a.tr.Keys ==> k.0 < a.numStates
-                                       && forall k:: k in a.tr.Values ==> k < a.numStates
-    witness Auto(0, map[], 0)
+  type ValidAuto = a: Auto | a.IsValid() witness Auto(0, map[])
 
-  //   function Union<T>(tr1: Transitions, tr2: Transitions, s1: nat, s2: nat, lastState: nat, computedStates: map<(Option<nat>, Option<nat>), nat>): map<(Option<nat>, Option<nat>), nat>
-  //   {
-  //     //  get successors of s1 and s2 on false
-  //     match SuccProd(s1, s2, false)
-  //         case (None, None) => computedStates
-  //         case (Some(k), None) => Union(tr1, [], k, )
-  //         case (None, Some(k)) =>
-  //         case (Some(k), Some(k')) =>
-  //     // var succ1, succ2 := Succ(s1, tr1), Succ(s2, tr2);
-  //     //  False successors
-  //     // match (succ1.0, succ2.0)
-  //     //     case (None, None) => computed
-  //     //     case (Some(k), None) => computed + Unfold()
-  //     //     case (None, Some(k)) => tr1
-  //     //     case (Some(k), Some(k')) => tr1
-  //     //     case  => tr1
-  //     // tr1
-  //   }
+  //   type NatAuto = ValidAuto<nat, bool> // witness Auto([], [], map[])
 
-  function Succ(s: nat, tr: Transitions, exit: bool): Option<nat>
+  type ValidPair = p: Pair | p.IsValid() witness Pair(Auto(1, map[]), Partition(1, [{0}]))
+
+  datatype Auto = Auto(numStates: nat, transitions: map<(nat, bool), nat>)
   {
-    if (s, exit) in tr then Some(tr[(s, exit)])
-    else None
-  }
 
-  function UnionSucc(a1: ValidAuto, a2: ValidAuto, s1: Option<nat>, s2: Option<nat>, exit: bool): (r: (Option<nat>, Option<nat>))
-    ensures r.0.Some? ==> r.0.v < a1.numStates
-    ensures r.1.Some? ==> r.1.v < a2.numStates
-  {
-    var s1' := if s1.None? || ((s1.v, exit) !in a1.tr) then None else Some(a1.tr[(s1.v, exit)]);
-    var s2' := if s2.None? || ((s2.v, exit) !in a2.tr) then None else Some(a2.tr[(s2.v, exit)]);
-    (s1', s2')
-  }
-
-  method DFS(a1: ValidAuto, s1: nat := 0, seen: set<nat> := {}, maxIter: nat)
-    decreases maxIter
-  {
-    match Succ(s1, a1.tr, false) {
-      case None =>  //    Explore true branch
-
-      case Some(v) =>
-        if v !in seen && maxIter > 0 {
-          print "s", s1, " -- false -> ", "s", v, "\n";
-          DFS(a1, v, seen + { v }, maxIter - 1);
-        }
+    predicate IsValid()
+    {
+      forall k:: k in transitions ==> transitions[k] < numStates
     }
 
-    match Succ(s1, a1.tr, true) {
-      case None =>  //    Done
-
-      case Some(v) =>
-        if v !in seen && maxIter > 0 {
-          print "s", s1, " -- true -> ", "s", v, "\n";
-          DFS(a1, v, seen + { v }, maxIter - 1);
-        }
+    /**
+      *  Successor state of s via l.
+      *  @param  s   A state index.
+      *  @param  l   A label index.
+      *  @returns    The successor of s via l if exists of None otherwise.      
+      */
+    function Succ(s: nat, l: bool): Option<nat>
+      requires this.IsValid()
+      requires 0 <= s < numStates
+      ensures Succ(s, l).Some? ==> 0 <= Succ(s, l).v < numStates
+    {
+      if (s, l) in transitions then Some(transitions[(s, l)])
+      else None
     }
+
   }
 
-  function DFS2(a1: ValidAuto, s1: nat := 0, seen: set<nat> := {}, maxDepth: nat): (seq<(nat, bool, nat)>)
-    decreases maxDepth
-  {
-    if s1 in seen || maxDepth == 0 then []
-    else
-      //  DFS false
-      var leftSucc := Succ(s1, a1.tr, false);
-      var leftBranch :=
-        if leftSucc.Some? then
-          var l := DFS2(a1, leftSucc.v, seen + { s1 }, maxDepth - 1);
-          [(s1, false, leftSucc.v)] + l
-        else [];
+  datatype Pair = Pair(a: ValidAuto, p: ValidPartition) {
 
-      //  DFS right
-      var rightSucc := Succ(s1, a1.tr, true);
-      var rightBranch :=
-        if rightSucc.Some? then
-          var r := DFS2(a1, rightSucc.v, seen + { s1 }, maxDepth - 1);
-          [(s1, true, rightSucc.v)] + r
-        else [];
-      leftBranch + rightBranch
-  }
-
-  lemma foo606(s: set<nat>, k: nat)
-    requires forall e:: e in s ==> e <= k
-    ensures |s| <= k + 1
-  {
-    if |s| == 0 {
-
-    } else {
-      if k == 0 {
-        assert s == { 0 };
-      }
-      else if k in s {
-        foo606(s - { k }, k - 1);
-      } else {
-        var e: nat :| e in s;
-        assert e <= k - 1;
-        foo606(s - { e }, k - 1);
-      }
+    predicate IsValid()
+    {
+      a.numStates == p.n
     }
-  }
 
-  function DFS3(a1: ValidAuto, s1: nat := 0, seen: set<nat> := {}): (seq<(nat, bool, nat)>)
-    // decreases maxDepth
-    requires forall k:: k in seen ==> k < a1.numStates
-    requires |seen| <= a1.numStates + 1 //  Not necessary to explicitly add this one
-    decreases a1.numStates - |seen|
-  {
-    if s1 in seen then []
-    else
-      //  DFS false
-      var leftSucc := Succ(s1, a1.tr, false);
-      var leftBranch :=
-        if leftSucc.Some? then
-          foo606(seen + {s1}, a1.numStates);
-          assert |seen + {s1}| > |seen|;
-          var l := DFS3(a1, leftSucc.v, seen + { s1 });
-          [(s1, false, leftSucc.v)] + l
-        else [];
-
-      //  DFS right
-      var rightSucc := Succ(s1, a1.tr, true);
-      var rightBranch :=
-        if rightSucc.Some? then
-          foo606(seen + {s1}, a1.numStates);
-          assert |seen + {s1}| > |seen|;
-          var r := DFS3(a1, rightSucc.v, seen + { s1 });
-          [(s1, true, rightSucc.v)] + r
-        else [];
-      leftBranch + rightBranch
-  }
-
-
-  predicate IsBounded<T>(s: set<T>, k: nat)
-  {
-    |s| <= k
-  }
-
-  lemma foo202<T>(s: set<T>, u: set<T>, k: nat)
-    requires IsBounded(s, k)
-    requires u <= s
-    ensures IsBounded(u, k)
-  {
-    if s != {} && s != u {
-        var e :| e in s && e !in u;
-        foo202(s - {e}, u, k - 1);
+    function Refine(): ValidPartition
+        requires this.IsValid()
+    {
+        p
     }
-  } 
-
-  function DFS4(a1: ValidAuto, s1: nat := 0, seen: set<nat> := {}): (seq<(nat, bool, nat)>)
-    // decreases maxDepth
-    requires forall k:: k in seen ==> k < a1.numStates
-    requires |seen| <= a1.numStates + 1 //  Not necessary to explicitly add this one
-    decreases a1.numStates - |seen|
-  {
-    if s1 in seen then []
-    else
-      //  DFS false
-      var leftSucc := Succ(s1, a1.tr, false);
-      var leftBranch :=
-        if leftSucc.Some? then
-          foo606(seen + {s1}, a1.numStates);
-          assert |seen + {s1}| > |seen|;
-          var l := DFS3(a1, leftSucc.v, seen + { s1 });
-          [(s1, false, leftSucc.v)] + l
-        else [];
-
-      //  DFS right
-      var rightSucc := Succ(s1, a1.tr, true);
-      var rightBranch :=
-        if rightSucc.Some? then
-          foo606(seen + {s1}, a1.numStates);
-          assert |seen + {s1}| > |seen|;
-          var r := DFS3(a1, rightSucc.v, seen + { s1 });
-          [(s1, true, rightSucc.v)] + r
-        else [];
-      leftBranch + rightBranch
-  }
-
-  method {:main} Main() {
-    var tr1 := map[ (0, true) := 1, (1, false) := 0, (0, false) := 2, (2, true) := 0];
-    var a1: ValidAuto := Auto(3, tr1);
-
-    // DFS(a1, 0, {}, 10);
-
-    var r := DFS3(a1);
-    PrintToDot(r);
 
   }
 
-  method PrintEdges(xe: seq<(nat, bool, nat)>) {
-    if |xe| > 0 {
-      print "s", xe[0].0, " -> s", xe[0].2, " [label=", xe[0].1, "]\n";
-      PrintEdges(xe[1..]);
-    }
-  }
 
-  method PrintToDot(xe: seq<(nat, bool, nat)>) {
-    print "digraph CFG", "\n";
-    print "{", "\n";
-    PrintEdges(xe);
-    print "}", "\n";
-
-  }
 
 }
